src/riscv/Platform/MetricMinimal.v
@@ -62,6 +62,7 @@ Section Riscv.
     getPrivMode := liftL0 id getPrivMode;
     setPrivMode := liftL1 id setPrivMode;
     fence := liftL2 id fence;
+    logInstr := liftL1 id logInstr;
     endCycleNormal := liftL0 (addMetricInstructions 1) endCycleNormal;
     endCycleEarly{A} := liftL0 (addMetricInstructions 1) (@endCycleEarly _ _ _ _ _ A);
   }.
