src/riscv/Spec/Primitives.v
@@ -92,6 +92,7 @@ Section Primitives.
     getPrivMode_sane: mcomp_sane getPrivMode;
     setPrivMode_sane: forall m, mcomp_sane (setPrivMode m);
     fence_sane: forall a b, mcomp_sane (fence a b);
+    logInstr_sane : forall a, mcomp_sane (logInstr a);  
     getPC_sane: mcomp_sane getPC;
     setPC_sane: forall newPc, mcomp_sane (setPC newPc);
     endCycleNormal_sane: mcomp_sane endCycleNormal;
